loop max example done

example_loop_max.thy
@@ -42,22 +42,44 @@ end
 
 type_synonym operation = unit
 
+datatype proc =
+    PMax "nat list"
 
-definition max_impl :: "val \<Rightarrow> (val,operation,val) io" where
+definition "only_store_changed PS_old PS \<equiv> \<exists>store'. PS = PS_old\<lparr>ps_store := store'\<rparr>"
+
+lemma show_only_store_changed:
+  assumes "only_store_changed PS_old PS"
+    and "PS' = PS\<lparr>ps_store := x\<rparr>"
+  shows "only_store_changed PS_old PS'"
+  using assms by (auto simp add: only_store_changed_def)
+
+definition loop_inv :: "nat list ref \<Rightarrow> nat ref \<Rightarrow> nat list \<Rightarrow> (proc, val, unit) proof_state \<Rightarrow> (proc, val, unit) proof_state \<Rightarrow> bool" where
+"loop_inv listR resR p_list PS_old PS \<equiv>
+ \<exists>li re li_done.
+          iref resR \<noteq> iref listR
+        \<and> (iref listR) \<in> dom (ps_store PS)
+        \<and> (iref resR) \<in> dom (ps_store PS)
+        \<and> li ::= s_read (ps_store PS) listR 
+        \<and> re ::= s_read (ps_store PS) resR 
+        \<and> p_list ::= li_done @ li
+        \<and> (if li_done = [] then re = 0 else re = Max (set li_done))
+        \<and> (only_store_changed PS_old PS)"
+
+definition max_impl :: "nat list \<Rightarrow> (val,operation,val) io" where
 "max_impl p_list \<equiv> 
    do {
-      listR \<leftarrow> makeRef (map nat_value (list_value p_list));
+      listR \<leftarrow> makeRef p_list;
       resR \<leftarrow> makeRef 0;
-      loop (do {
+      loop_a (loop_inv listR resR p_list) (do {
         list \<leftarrow> read listR;
         res \<leftarrow> read resR;
         if list = [] then 
-          return False
+          return True
         else do {
           let x = hd list;
-          listR ::= tl list;
-          resR ::= max x res;
-          return True
+          listR :\<leftarrow> tl list;
+          resR :\<leftarrow> max x res;
+          return False
         }
       });
       res \<leftarrow> read resR;
@@ -66,8 +88,7 @@ definition max_impl :: "val \<Rightarrow> (val,operation,val) io" where
 
 
 
-datatype proc =
-    PMax "nat list"
+
 
 instance proc :: countable
   by countable_datatype
@@ -89,7 +110,7 @@ type_synonym localState = "val store \<times> (val, operation, val) io"
 definition procedures :: "proc \<Rightarrow> (localState \<times> (localState, operation, val) procedureImpl)" where
   "procedures invoc \<equiv>
   case invoc of
-    PMax n \<Rightarrow> toImpl2 (max_impl (ListVal (map Nat n)))
+    PMax n \<Rightarrow> toImpl2 (max_impl n)
 "
 
 
@@ -132,7 +153,7 @@ proof (auto simp add: program_wellFormed_def)
   proof (auto simp add: procedures_cannot_guess_ids_def procedures_def uniqueIds_proc_def split: proc.splits)
 
     show "\<And>x uids.
-       procedure_cannot_guess_ids uids (Map.empty, max_impl (ListVal (map val.Nat x))) impl_language_loops.toImpl "
+       procedure_cannot_guess_ids uids (Map.empty, max_impl x) impl_language_loops.toImpl "
       apply (auto simp add: max_impl_def, show_procedures_cannot_guess_ids)
       sorry
   qed
@@ -189,7 +210,7 @@ proof M_show_programCorrect
       next
         case execution
 
-        have ls: "localState S i \<triangleq> (Map.empty, max_impl (ListVal (map val.Nat list)))"
+        have ls: "localState S i \<triangleq> (Map.empty, max_impl list)"
             by (auto simp add: PMax procedures_def )
 
         show "execution_s_correct S i"
@@ -207,6 +228,11 @@ proof M_show_programCorrect
 
           show "program_wellFormed (prog S)"
             by (auto simp add: show_P)
+
+          from `invariant_all' S`
+          show "invariant progr (invariantContext.truncate S)"
+            unfolding invContext'_truncate by auto
+
 
 
           show "program_proof_rules_loops.execution_s_check (invariant progr) (querySpec progr) \<lparr>
@@ -227,769 +253,79 @@ proof M_show_programCorrect
                   ps_firstTx = True, 
                   ps_store = Map.empty
                   \<rparr> 
-                  (max_impl (ListVal (map val.Nat list))) 
+                  (max_impl list) 
                   (finalCheck inv i)" \<comment> \<open>TODO finalCheck could be fixed for the initial P (as variant)\<close>
             if c0: "(\<And>tx. s_transactionOrigin tx \<noteq> Some i)"
+              and inv: "invariant progr
+                         \<lparr>calls = s_calls, happensBefore = s_happensBefore, callOrigin = s_callOrigin,
+                            transactionOrigin = s_transactionOrigin, knownIds = s_knownIds,
+                            invocationOp = s_invocationOp(i \<mapsto> PMax list), invocationRes = s_invocationRes(i := None)\<rparr>"
             for  s_calls s_happensBefore s_callOrigin s_transactionOrigin s_knownIds s_invocationOp s_invocationRes
             apply (auto simp add: )
-            apply repliss_vcg_l
-
-
-          show "\<And>s_calls s_happensBefore s_callOrigin s_transactionOrigin s_knownIds s_invocationOp s_invocationRes.
-       (\<And>tx. s_transactionOrigin tx \<noteq> Some i) \<Longrightarrow>
-       program_proof_rules_loops.execution_s_check (invariant progr) (querySpec progr)
-        \<lparr>calls = s_calls, happensBefore = s_happensBefore, callOrigin = s_callOrigin,
-           transactionOrigin = s_transactionOrigin, knownIds = s_knownIds,
-           invocationOp = s_invocationOp(i \<mapsto> PMax list), invocationRes = s_invocationRes(i := None), ps_i = i,
-           ps_generatedLocal = {}, ps_generatedLocalPrivate = {}, ps_localKnown = uniqueIds (PMax list), ps_vis = {},
-           ps_localCalls = [], ps_tx = None, ps_firstTx = True, ps_store = Map.empty\<rparr>
-        (max_impl (ListVal (map val.Nat list))) ?P"
-
-
-          show "execution_s_check progr i s_calls s_happensBefore s_callOrigin s_transactionOrigin s_knownIds (s_invocationOp(i \<mapsto> SendMessage author content)) (s_invocationRes(i := None)) {} {} {} [] None True (sendMessage_impl (String author) (String content))"
-            if tx_fresh: "(\<And>tx. s_transactionOrigin tx \<noteq> Some i)"
-            for  s_calls s_happensBefore s_callOrigin s_transactionOrigin s_knownIds s_invocationOp s_invocationRes
-          proof (repliss_vcg, goal_cases "AtCommit" "AtReturn" )
-            case (AtCommit v tx s_calls' s_happensBefore' s_callOrigin' s_transactionOrigin' s_knownIds' vis' s_invocationOp' s_invocationRes' c res ca resa cb resb)
-
-            have [simp]: "res = Undef"
-              using local.AtCommit(16)
-              by (auto simp add: crdtSpec_def struct_field_def map_dw_spec_def map_spec_def messageStruct_def register_spec_def)
-            have [simp]:"resa = Undef"
-              using local.AtCommit(17)
-              by (auto simp add: crdtSpec_def struct_field_def map_dw_spec_def map_spec_def messageStruct_def register_spec_def)
-
-            have [simp]:"resb = Undef"
-              using local.AtCommit(18)
-              by (auto simp add: crdtSpec_def struct_field_def set_rw_spec_def)
-
-            have [simp]:  "in_sequence [c, ca, cb] c ca"
-              by (simp add: in_sequence_cons)
-
-            have "new_unique_not_in_calls s_calls' (to_nat v)"
-              by (meson AtCommit(13) uid_is_private'_def)
-
-
-            hence no_v: "to_nat v \<notin> uniqueIds opr" if "s_calls' c \<triangleq> Call opr r" for c opr r
-              by (meson new_unique_not_in_calls_def that)
-
-            have [simp]: "s_calls' delete \<noteq> Some (Call (Message (DeleteKey v)) Undef)" for delete
-              apply auto
-              apply (drule no_v)
-             using `uniqueIds_val_r v = {to_nat v}` by auto
-
-            from AtCommit
+            apply (repliss_vcg_l asmUnfold: loop_inv_def)
+          proof (goal_cases loop_inv_start final loop_body )
+            case loop_inv_start
             show ?case
-            proof (auto simp add: inv_def, goal_cases  inv2 inv3 inv4)
-              case (inv2 some_generatedIds some_generatedIds1 some_currentTransaction some_currentTransaction1 some_localState some_localState1 some_currentProc some_currentProc1 some_visibleCalls some_visibleCalls1 some_transactionStatus some_transactionStatus1 some_generatedIds2 some_currentTransaction2 some_localState2 some_currentProc2 some_visibleCalls2 some_transactionStatus2)
-              then show ?case
-                by (auto simp add: inv2_def exists_cases1)
-
-            next
-              case (inv3 some_generatedIds some_generatedIds1 some_currentTransaction some_currentTransaction1 some_localState some_localState1 some_currentProc some_currentProc1 some_visibleCalls some_visibleCalls1 some_transactionStatus some_transactionStatus1 some_generatedIds2 some_currentTransaction2 some_localState2 some_currentProc2 some_visibleCalls2 some_transactionStatus2)
-              
-              from inv3 show ?case 
-                by (auto simp add: inv3_def updateHb_cases in_sequence_cons cong: conj_cong, meson)
-            next
-              case (inv4 some_generatedIds some_generatedIds1 some_currentTransaction some_currentTransaction1 some_localState some_localState1 some_currentProc some_currentProc1 some_visibleCalls some_visibleCalls1 some_transactionStatus some_transactionStatus1 some_generatedIds2 some_currentTransaction2 some_localState2 some_currentProc2 some_visibleCalls2 some_transactionStatus2)
-              then show ?case 
-                by (auto simp add: inv4_def is_update_operation_def in_sequence_cons updateHb_cases)
-            qed
-              
-              
+              unfolding loop_inv_def
+              by (auto simp add: s_read_def Def_def only_store_changed_def)
           next
-            case (AtReturn v tx s_calls' s_happensBefore' s_callOrigin' s_transactionOrigin' s_knownIds' vis' s_invocationOp' s_invocationRes' c res ca resa cb resb)
-            then show ?case
-              apply (auto simp add: inv_def)
-              apply (auto simp add: inv1_def)
-              by (smt map_upd_Some_unfold proc.inject(1))
+            case (loop_body PS li_v li re_v re li_done)
+            have [simp]: "fromAny li_v = li"
+              using loop_body by (auto simp add: Def_def s_read_def)
 
-          qed
+            have [simp]: "fromAny re_v = re"
+              using loop_body by (auto simp add: Def_def s_read_def)
 
-        qed
-      qed
+            have "li \<noteq> []"
+              using loop_body Def_def by metis
 
-    next
-      case (EditMessage m newContent)
-      show "procedureCorrect progr S i"
-      proof M_show_procedureCorrect
-        case after_invocation
-        show ?case
-          using show_P.invariant_pre EditMessage show_P.i_fresh
-          by (auto simp add:  inv_def inv1_def inv2_def inv3_def inv4_def invContextH2_simps, 
-              metis option.distinct(1) show_P.i_fresh)+
-
-      next
-        case execution
-
-        show "execution_s_correct progr S i"
-          using procedure_correct.in_initial_state
-        proof (fuzzy_rule execution_s_check_sound3)
-          show "currentProc S i \<triangleq> toImpl"
-            by (auto simp add: EditMessage procedures_def )
-
-          show "localState S i \<triangleq> editMessage_impl (MessageId m) (String newContent)"
-            by (auto simp add: EditMessage procedures_def )
-
-          show "invocationOp S i \<triangleq> EditMessage m newContent"
-            using EditMessage \<open>invocationOp S i \<triangleq> proc\<close> by blast
-
-          note editMessage_impl_def[simp]
-
-          
-
-          show "execution_s_check progr i s_calls s_happensBefore s_callOrigin s_transactionOrigin s_knownIds (s_invocationOp(i \<mapsto> EditMessage m newContent)) (s_invocationRes(i := None)) {} {} {} [] None True (editMessage_impl (MessageId m) (String newContent))"
-            if tx_fresh: "(\<And>tx. s_transactionOrigin tx \<noteq> Some i)"
-            for  s_calls s_happensBefore s_callOrigin s_transactionOrigin s_knownIds s_invocationOp s_invocationRes
-          proof (repliss_vcg, goal_cases "Exists_AtCommit" "Exists_AtReturn" "NotExists_AtCommit" "NotExists_AtReturn")
-            case (Exists_AtCommit tx s_calls' s_happensBefore' s_callOrigin' s_transactionOrigin' s_knownIds' vis' s_invocationOp' s_invocationRes' c res ca resa)
-
-            note `c \<noteq> ca`[simp]
-
-            from `example_chat.inv
-             \<lparr>calls = s_calls', happensBefore = s_happensBefore', callOrigin = s_callOrigin', transactionOrigin = s_transactionOrigin',
-                knownIds = s_knownIds', invocationOp = s_invocationOp'(i \<mapsto> EditMessage m newContent),
-                invocationRes = s_invocationRes'(i := None)\<rparr>`
-            have  i1: "inv1 (s_invocationOp'(i \<mapsto> EditMessage m newContent)) (s_invocationRes'(i := None))"
-              and i2: "inv2 (s_invocationOp'(i \<mapsto> EditMessage m newContent)) s_calls'"
-              and i3: "inv3 s_calls' s_happensBefore'"
-              and i4: "inv4 s_calls' s_happensBefore'"
-              by (auto simp add: inv_def)
-
-            from \<open>crdtSpec (Message (KeyExists (MessageId m))) \<lparr>calls = s_calls' |` vis', happensBefore = s_happensBefore' |r vis'\<rparr> (Bool True)\<close>
-            obtain upd_c upd_op upd_r
-              where upd_vis: "upd_c \<in> vis'"
-                and upd_call: "s_calls' upd_c \<triangleq> Call (Message (NestedOp (MessageId m) upd_op)) upd_r"
-                and upd_is_update: "is_update upd_op"
-                and ipd_not_deleted: "\<forall>c'. c' \<in> vis' \<longrightarrow> (\<forall>x2. s_calls' c' \<triangleq> x2 \<longrightarrow> (\<forall>x2a. x2 \<noteq> Call (Message (DeleteKey (MessageId m))) x2a) \<or> (c', upd_c) \<in> s_happensBefore')"
-              by (auto simp add: crdtSpec_def struct_field_def map_dw_spec_def map_spec_def restrict_ctxt_op_def restrict_ctxt_def fmap_map_values_def'
-                      restrict_map_def deleted_calls_dw_def restrict_relation_def
-                   split: option.splits if_splits operation.splits call.splits)
-
-
-
-
-
-            hence "upd_r = Undef"
-              using Exists_AtCommit(9) query_result_undef by auto
-
-
-            have "upd_c \<noteq> c"
-              by (smt Exists_AtCommit(15) Exists_AtCommit(5) Exists_AtCommit(9) basic_trans_rules(31) domIff invariantContext.simps(1) operationContext.select_convs(1) upd_vis wellFormed_callOrigin_dom3)
-
-            have "upd_c \<noteq> ca"
-              by (smt Exists_AtCommit(15) Exists_AtCommit(5) Exists_AtCommit(9) basic_trans_rules(31) domIff invariantContext.simps(1) operationContext.select_convs(1) upd_vis wellFormed_callOrigin_dom)
-
-            obtain upda_c upda_val
-              where upda_call: "s_calls' upda_c \<triangleq> Call (Message (NestedOp (MessageId m) (Author (Assign upda_val)))) Undef"
-                and upda_before_upd: "(upda_c, upd_c) \<in> s_happensBefore' \<or> upda_c = upd_c"
-            proof (atomize_elim, cases upd_op)
-              case (Author a)
-              obtain x where "a = Assign x"
-                using upd_is_update Author 
-                by (cases a, auto simp add: is_update_messageDataOp_def)
-
-              show "\<exists>upda_c upda_val.
-                   s_calls' upda_c \<triangleq> Call (Message (NestedOp (MessageId m) (Author (Assign upda_val)))) Undef \<and>
-                   ((upda_c, upd_c) \<in> s_happensBefore' \<or> upda_c = upd_c)"
-                using Author \<open>a = Assign x\<close> upd_call \<open>upd_r = Undef\<close> by blast
-
-            next
-              case (Content a)
-              obtain x where "a = Assign x"
-                using upd_is_update Content 
-                by (cases a, auto simp add: is_update_messageDataOp_def)
-
-              show "\<exists>upda_c upda_val.
-                 s_calls' upda_c \<triangleq> Call (Message (NestedOp (MessageId m) (Author (Assign upda_val)))) Undef \<and>
-                 ((upda_c, upd_c) \<in> s_happensBefore' \<or> upda_c = upd_c)"
-                using i3 Content \<open>a = Assign x\<close> \<open>upd_r = Undef\<close> upd_call 
-                by (auto simp add: inv3_def, blast)
-            qed
-
-
-
-            have "upda_c \<noteq> c"
-              using Exists_AtCommit \<open>upd_c \<noteq> c\<close> upda_before_upd by blast
-
-            have "upda_c \<noteq> ca"
-              using Exists_AtCommit \<open>upd_c \<noteq> ca\<close> upda_before_upd by blast
-
-
-
-
-
-            from Exists_AtCommit
-            show ?case
-            proof (auto simp add: inv_def, goal_cases "inv2" "inv3" "inv4" )
-              case (inv2 some_generatedIds some_generatedIds1 some_currentTransaction some_currentTransaction1 some_localState some_localState1 some_currentProc some_currentProc1 some_visibleCalls some_visibleCalls1 some_transactionStatus some_transactionStatus1 some_generatedIds2 some_currentTransaction2 some_localState2 some_currentProc2 some_visibleCalls2 some_transactionStatus2)
-              then show ?case 
-                by (auto simp add: inv2_def)
-            next
-              case (inv3 some_generatedIds some_generatedIds1 some_currentTransaction some_currentTransaction1 some_localState some_localState1 some_currentProc some_currentProc1 some_visibleCalls some_visibleCalls1 some_transactionStatus some_transactionStatus1 some_generatedIds2 some_currentTransaction2 some_localState2 some_currentProc2 some_visibleCalls2 some_transactionStatus2)
-              show ?case 
-                apply (auto simp add: inv3_def updateHb_cases in_sequence_cons cong: conj_cong)
-                 apply (rule exI[where x=upda_c])
-                 apply (auto simp add: \<open>upda_c \<noteq> c\<close> \<open>upda_c \<noteq> ca\<close> upda_call)
-                using causallyConsistent_def inv3(6) upd_vis upda_before_upd apply fastforce
-                by (metis i3 inv3(13) inv3_def)
-            next
-              case (inv4 some_generatedIds some_generatedIds1 some_currentTransaction some_currentTransaction1 some_localState some_localState1 some_currentProc some_currentProc1 some_visibleCalls some_visibleCalls1 some_transactionStatus some_transactionStatus1 some_generatedIds2 some_currentTransaction2 some_localState2 some_currentProc2 some_visibleCalls2 some_transactionStatus2)
-              then show ?case 
-                apply (auto simp add: inv4_def updateHb_cases in_sequence_cons)
-                by (metis (no_types, lifting) \<open>upd_r = Undef\<close> ipd_not_deleted upd_call upd_is_update)
-            qed
-              
-          next
-            case (Exists_AtReturn tx s_calls' s_happensBefore' s_callOrigin' s_transactionOrigin' s_knownIds' vis' s_invocationOp' s_invocationRes' c res ca resa)
-            then show ?case 
-              apply (auto simp add: inv_def )
-              apply (auto simp add: inv1_def cong: conj_cong)
-              by (smt map_upd_Some_unfold proc.distinct(1))
-          next
-            case (NotExists_AtCommit tx s_calls' s_happensBefore' s_callOrigin' s_transactionOrigin' s_knownIds' vis' s_invocationOp' s_invocationRes' c res)
-            then show ?case 
-            proof (auto simp add: inv_def, goal_cases inv2 inv3 inv4)
-              case (inv2 some_generatedIds some_generatedIds1 some_currentTransaction some_currentTransaction1 some_localState some_localState1 some_currentProc some_currentProc1 some_visibleCalls some_visibleCalls1 some_transactionStatus some_transactionStatus1 some_generatedIds2 some_currentTransaction2 some_localState2 some_currentProc2 some_visibleCalls2 some_transactionStatus2)
-              then show ?case by (auto simp add: inv2_def)
-            next
-              case (inv3 some_generatedIds some_generatedIds1 some_currentTransaction some_currentTransaction1 some_localState some_localState1 some_currentProc some_currentProc1 some_visibleCalls some_visibleCalls1 some_transactionStatus some_transactionStatus1 some_generatedIds2 some_currentTransaction2 some_localState2 some_currentProc2 some_visibleCalls2 some_transactionStatus2)
-              then show ?case by (auto simp add: inv3_def updateHb_single cong: conj_cong, fastforce)
-            next
-              case (inv4 some_generatedIds some_generatedIds1 some_currentTransaction some_currentTransaction1 some_localState some_localState1 some_currentProc some_currentProc1 some_visibleCalls some_visibleCalls1 some_transactionStatus some_transactionStatus1 some_generatedIds2 some_currentTransaction2 some_localState2 some_currentProc2 some_visibleCalls2 some_transactionStatus2)
-              then show ?case 
-                by (auto simp add: inv4_def updateHb_single)
-            qed
-          next
-            case (NotExists_AtReturn tx s_calls' s_happensBefore' s_callOrigin' s_transactionOrigin' s_knownIds' vis' s_invocationOp' s_invocationRes' c res)
-            then show ?case 
-              apply (auto simp add: inv_def inv1_def cong: conj_cong)
-              by (meson option.inject proc.simps(6))
-          qed
-        qed
-      qed
-    next
-      case (DeleteMessage m)
-
-
-      show "procedureCorrect progr S i"
-      proof M_show_procedureCorrect
-        case after_invocation
-        show ?case
-          using show_P.invariant_pre DeleteMessage show_P.i_fresh
-          by (auto simp add:  inv_def inv1_def inv2_def inv3_def inv4_def invContextH2_simps, 
-              metis option.distinct(1) show_P.i_fresh)+
-
-      next
-        case execution
-
-        show "execution_s_correct progr S i"
-          using procedure_correct.in_initial_state
-        proof (fuzzy_rule execution_s_check_sound3)
-          show "currentProc S i \<triangleq> toImpl"
-            by (auto simp add: DeleteMessage procedures_def )
-
-          show "localState S i \<triangleq> deleteMessage_impl (MessageId m)"
-            by (auto simp add: DeleteMessage procedures_def )
-
-          show "invocationOp S i \<triangleq> DeleteMessage m"
-            using DeleteMessage \<open>invocationOp S i \<triangleq> proc\<close> by blast
-
-          note deleteMessage_impl_def[simp]
-
-          show "execution_s_check progr i s_calls s_happensBefore s_callOrigin s_transactionOrigin s_knownIds (s_invocationOp(i \<mapsto> DeleteMessage m)) (s_invocationRes(i := None)) {} {} {} [] None True (deleteMessage_impl (MessageId m))"
-            if tx_fresh: "(\<And>tx. s_transactionOrigin tx \<noteq> Some i)"
-            for  s_calls s_happensBefore s_callOrigin s_transactionOrigin s_knownIds s_invocationOp s_invocationRes
-          proof (repliss_vcg, goal_cases "Exists_AtCommit" "Exists_AtReturn" "NotExists_AtCommit" "NotExists_AtReturn")
-            case (Exists_AtCommit tx s_calls' s_happensBefore' s_callOrigin' s_transactionOrigin' s_knownIds' vis' s_invocationOp' s_invocationRes' c res ca resa cb resb)
-
-            from `c \<noteq> ca \<and> c \<noteq> cb \<and> ca \<noteq> cb`
-            have [simp]: "c \<noteq> ca" "c \<noteq> cb" "ca \<noteq> cb"
-              by auto
-
-
-            from `example_chat.inv
-               \<lparr>calls = s_calls', happensBefore = s_happensBefore', callOrigin = s_callOrigin', transactionOrigin = s_transactionOrigin',
-                  knownIds = s_knownIds', invocationOp = s_invocationOp'(i \<mapsto> DeleteMessage m), invocationRes = s_invocationRes'(i := None)\<rparr>`
-            have  i1: "inv1 (s_invocationOp'(i \<mapsto> DeleteMessage m)) (s_invocationRes'(i := None))"
-              and i2: "inv2 (s_invocationOp'(i \<mapsto> DeleteMessage m)) s_calls'"
-              and i3: "inv3 s_calls' s_happensBefore'"
-              and i4: "inv4 s_calls' s_happensBefore'"
-              by (auto simp add: inv_def)
 
             show ?case
-            proof (auto simp add: inv_def, goal_cases inv1 inv2 inv3 inv4)
-              case inv1
-              from i1
-              show ?case by auto
-            next
-              case inv2
-              from i2
-              show ?case
-                by (auto simp add: inv2_def)
-            next
-              case inv3
-              from i3
-              show ?case 
-                apply (auto simp add: inv3_def updateHb_cases cong: conj_cong)
-                by (metis Exists_AtCommit(18)) 
+              unfolding loop_inv_def
+              apply (rule exI[where x="tl li"])
+              apply (rule exI[where x="max (hd li) re"])
+              apply (rule exI[where x="li_done @ [hd li]"])
+            proof (auto simp add: Def_def loop_body s_read_def intro!: show_only_store_changed[OF loop_body(7)])
+              show "list = li_done @ hd li # tl li"
+                using Def_def \<open>li \<noteq> []\<close> `list ::= li_done @ li` by fastforce
 
-            next
-              case inv4
-              then show ?case
-                apply (auto simp add: inv4_def updateHb_cases in_sequence_cons)
-                using Exists_AtCommit(18) apply blast
-                by (meson i4 inv4_def)
+              from `if li_done = [] then re = 0 else re = Max (set li_done)`
+              show "max (hd li) re = Max (insert (hd li) (set li_done))"
+                by (auto split: if_splits)
             qed
-              
-          next
-            case (Exists_AtReturn tx s_calls' s_happensBefore' s_callOrigin' s_transactionOrigin' s_knownIds' vis' s_invocationOp' s_invocationRes' c res ca resa cb resb)
-            then show ?case
-              apply (auto simp add: inv_def inv1_def)
-              by (metis (no_types, lifting) option.inject proc.distinct(3))
-          next
-            case (NotExists_AtCommit tx s_calls' s_happensBefore' s_callOrigin' s_transactionOrigin' s_knownIds' vis' s_invocationOp' s_invocationRes' c res)
-            then show ?case
-            proof (auto simp add: inv_def, goal_cases inv2 inv3 inv4)
-              case (inv2 some_generatedIds some_generatedIds1 some_currentTransaction some_currentTransaction1 some_localState some_localState1 some_currentProc some_currentProc1 some_visibleCalls some_visibleCalls1 some_transactionStatus some_transactionStatus1 some_generatedIds2 some_currentTransaction2 some_localState2 some_currentProc2 some_visibleCalls2 some_transactionStatus2)
-              then show ?case
-                by (auto simp add: inv2_def)
-            next
-              case (inv3 some_generatedIds some_generatedIds1 some_currentTransaction some_currentTransaction1 some_localState some_localState1 some_currentProc some_currentProc1 some_visibleCalls some_visibleCalls1 some_transactionStatus some_transactionStatus1 some_generatedIds2 some_currentTransaction2 some_localState2 some_currentProc2 some_visibleCalls2 some_transactionStatus2)
-              then show ?case 
-                by (auto simp add: inv3_def updateHb_cases in_sequence_cons, fastforce)
 
-            next
-              case (inv4 some_generatedIds some_generatedIds1 some_currentTransaction some_currentTransaction1 some_localState some_localState1 some_currentProc some_currentProc1 some_visibleCalls some_visibleCalls1 some_transactionStatus some_transactionStatus1 some_generatedIds2 some_currentTransaction2 some_localState2 some_currentProc2 some_visibleCalls2 some_transactionStatus2)
-              then show ?case 
-                by (auto simp add: inv4_def updateHb_cases in_sequence_cons)
-            qed
           next
-            case (NotExists_AtReturn tx s_calls' s_happensBefore' s_callOrigin' s_transactionOrigin' s_knownIds' vis' s_invocationOp' s_invocationRes' c res)
-            then show ?case 
-              apply (auto simp add: inv_def inv1_def)
-              by (metis (no_types, lifting) option.inject proc.distinct(3)) 
+            case (final PS li_v li re_v re li_done)
+            show ?case
+            proof (auto simp add: inv_def inv1_def invariantContext.defs)
+
+              show "s_read (ps_store PS) (Ref (Suc 0)) = Max (set list)"
+                if c0: "invocationOp PS i \<triangleq> PMax list"
+                  and c1: "list \<noteq> []"
+                for  list
+                using final that by (auto simp add: inv_def inv1_def invariantContext.defs Def_def only_store_changed_def split: if_splits)
+                               
+
+              show "r = val.Nat (Max (set list))"
+                if c0: "ia \<noteq> i"
+                  and c1: "invocationOp PS ia \<triangleq> PMax list"
+                  and c2: "list \<noteq> []"
+                  and c3: "invocationRes PS ia \<triangleq> r"
+                for  ia list r
+                using inv that final(7)
+                by (auto simp add: inv_def inv1_def final(7) only_store_changed_def, force)
+            qed
           qed
-        qed
-      qed
-    next
-      case (GetMessage m)
 
 
-      show "procedureCorrect progr S i"
-      proof M_show_procedureCorrect
-        case after_invocation
-        show ?case
-          using show_P.invariant_pre GetMessage show_P.i_fresh
-        proof (auto simp add:  inv_def invContextH2_simps, goal_cases inv1 inv2)
-          case inv1
-          then show ?case
-            apply (auto simp add: inv1_def state_wellFormed_invocation_before_result)
-            by (metis option.simps(3) show_P.i_fresh)
-        next
-          case inv2
-          then show ?case
-            apply (auto simp add: inv2_def)
-            by (metis option.distinct(1) show_P.i_fresh)
-        qed
 
-      next
-        case execution
 
-        show "execution_s_correct progr S i"
-          using procedure_correct.in_initial_state
-        proof (fuzzy_rule execution_s_check_sound3)
-          show "currentProc S i \<triangleq> toImpl"
-            by (auto simp add: GetMessage procedures_def )
-
-          show "localState S i \<triangleq> getMessage_impl (MessageId m)"
-            by (auto simp add: GetMessage procedures_def )
-
-          show "invocationOp S i \<triangleq> GetMessage m"
-            using GetMessage \<open>invocationOp S i \<triangleq> proc\<close> by blast
-
-          note getMessage_impl_def[simp]
-
-          show "execution_s_check progr i s_calls s_happensBefore s_callOrigin s_transactionOrigin s_knownIds (s_invocationOp(i \<mapsto> GetMessage m)) (s_invocationRes(i := None)) {} {} {} [] None True (getMessage_impl (MessageId m))"
-            if tx_fresh: "(\<And>tx. s_transactionOrigin tx \<noteq> Some i)"
-            for  s_calls s_happensBefore s_callOrigin s_transactionOrigin s_knownIds s_invocationOp s_invocationRes
-          proof (repliss_vcg, goal_cases "Exists_AtCommit" "Exists_AtReturn" "NotExists_AtCommit" "NotExists_AtReturn")
-            case (Exists_AtCommit tx s_calls' s_happensBefore' s_callOrigin' s_transactionOrigin' s_knownIds' vis' s_invocationOp' s_invocationRes' c res ca resa cb resb)
-            then show ?case 
-            proof (auto simp add: inv_def, goal_cases inv2 inv3 inv4)
-              case (inv2 some_generatedIds some_generatedIds1 some_currentTransaction some_currentTransaction1 some_localState some_localState1 some_currentProc some_currentProc1 some_visibleCalls some_visibleCalls1 some_transactionStatus some_transactionStatus1 some_generatedIds2 some_currentTransaction2 some_localState2 some_currentProc2 some_visibleCalls2 some_transactionStatus2)
-              then show ?case 
-                by (auto simp add: inv2_def)
-            next
-              case (inv3 some_generatedIds some_generatedIds1 some_currentTransaction some_currentTransaction1 some_localState some_localState1 some_currentProc some_currentProc1 some_visibleCalls some_visibleCalls1 some_transactionStatus some_transactionStatus1 some_generatedIds2 some_currentTransaction2 some_localState2 some_currentProc2 some_visibleCalls2 some_transactionStatus2)
-              then show ?case 
-                by (auto simp add: inv3_def  updateHb_cons cong: conj_cong, meson)
-            next
-              case (inv4 some_generatedIds some_generatedIds1 some_currentTransaction some_currentTransaction1 some_localState some_localState1 some_currentProc some_currentProc1 some_visibleCalls some_visibleCalls1 some_transactionStatus some_transactionStatus1 some_generatedIds2 some_currentTransaction2 some_localState2 some_currentProc2 some_visibleCalls2 some_transactionStatus2)
-              then show ?case 
-                by (auto simp add: inv4_def updateHb_cons is_update_messageDataOp_def)
-            qed  
-          next
-            case (Exists_AtReturn tx s_calls' s_happensBefore' s_callOrigin' s_transactionOrigin' s_knownIds' vis' s_invocationOp' s_invocationRes' c res ca resa cb resb)
-            
-            from \<open>example_chat.inv
-             \<lparr>calls = s_calls', happensBefore = s_happensBefore', callOrigin = s_callOrigin',
-                transactionOrigin = s_transactionOrigin', knownIds = s_knownIds',
-                invocationOp = s_invocationOp'(i \<mapsto> GetMessage m), invocationRes = s_invocationRes'(i := None)\<rparr>\<close>
-            have i1: "inv1 (s_invocationOp'(i \<mapsto> GetMessage m)) (s_invocationRes'(i := None))"
-              and i2: "inv2 (s_invocationOp'(i \<mapsto> GetMessage m)) s_calls'"
-              and i3: "inv3 s_calls' s_happensBefore'"
-              and i4: "inv4 s_calls' s_happensBefore'"
-              by (auto simp add: inv_def)
-
-            have "c \<notin> vis'"
-              by (simp add: Exists_AtReturn(17))
-
-
-
-            from Exists_AtReturn show ?case
-            proof (auto simp add: inv_def, goal_cases inv1)
-              case (inv1 some_generatedIds some_generatedIds1 some_currentTransaction some_currentTransaction1 some_localState some_localState1 some_currentProc some_currentProc1 some_visibleCalls some_visibleCalls1 some_transactionStatus some_transactionStatus1 some_generatedIds2 some_currentTransaction2 some_localState2 some_currentProc2 some_visibleCalls2 some_transactionStatus2)
-
-              
-
-              show ?case
-              proof (auto simp add: inv1_def cong: conj_cong)
-
-                show "\<exists>s. s \<noteq> i \<and> (\<exists>content2. s_invocationOp' s \<triangleq> SendMessage author content2)"
-                  if c0: "g \<noteq> i"
-                    and c1: "s_invocationOp' g \<triangleq> GetMessage m'"
-                    and c2: "s_invocationRes' g \<triangleq> Found (String author) content"
-                  for  g m' author content
-                  using \<open>inv1 (s_invocationOp'(i \<mapsto> GetMessage m)) (s_invocationRes'(i := None))\<close>
-                  using that apply (auto simp add: inv1_def)
-                  by (metis option.inject proc.distinct(5))
-
-
-                show "\<exists>s. s \<noteq> i \<and> (\<exists>content2. s_invocationOp' s \<triangleq> SendMessage author content2)"
-                  if c0: "resa = String author"
-                  for  author
-                proof -
-
-                  have [simp]: "x \<in> Field (s_happensBefore' |r vis') \<Longrightarrow> x \<in> vis'" for x
-                    by (auto simp add: Field_def restrict_relation_def)
-
-                  hence [simp]: " x \<in> Field (s_happensBefore' |r vis') \<Longrightarrow> \<exists>y. s_calls' x \<triangleq> y" for x
-                    by (meson  in_dom `vis' \<subseteq> dom s_calls'`)
-
-                  from \<open>crdtSpec (Message (KeyExists (MessageId m)))
-                     \<lparr>calls = s_calls' |` vis', happensBefore = s_happensBefore' |r vis'\<rparr> (Bool True)\<close>
-                  have "crdtSpec' (Message (KeyExists (MessageId m))) (dom s_calls' \<inter> vis') (extract_op s_calls') s_happensBefore' id (Bool True)"
-                    apply (subst(asm) crdtSpec'_alt)
-                    by (auto simp add: crdtSpec'_alt crdtSpec'_simp_op crdtSpec'_simp_hb)
-
-
-
-                  from this
-                  obtain upd_c upd_call upd_op
-                    where upd_call1: "s_calls' upd_c \<triangleq> upd_call"
-                      and upd_vis: "upd_c \<in> vis'"
-                      and upd_c_op: "extract_op s_calls' upd_c = Message (NestedOp (MessageId m) upd_op)"
-                      and upd_is_update: "is_update upd_op"
-                      and ud_not_deleted: "\<forall>d. extract_op s_calls' d = Message (DeleteKey (MessageId m)) \<longrightarrow> d \<in> dom s_calls' \<and> d \<in> vis' \<longrightarrow> (d, upd_c) \<in> s_happensBefore'"
-                    by (auto simp add: C_out_calls_def crdtSpec'_def struct_field'_def map_dw_spec'_def map_spec'_def deleted_calls_dw'_def)
-
-                  obtain upd_r where 
-                    upd_call: "s_calls' upd_c \<triangleq> Call (Message (NestedOp (MessageId m) upd_op)) upd_r"
-                    using upd_call1 upd_c_op
-                    by (auto simp add: extract_op_def' split: call.splits)
-
-
-                  have "upd_r = Undef"
-                    using local.Exists_AtReturn(9) upd_call upd_is_update
-                    by (rule query_result_undef)
-
-
-                  obtain upda_c upda_val
-                    where upda_call: "s_calls' upda_c \<triangleq> Call (Message (NestedOp (MessageId m) (Author (Assign upda_val)))) Undef"
-                      and upda_before_upd: "(upda_c, upd_c) \<in> s_happensBefore' \<or> upda_c = upd_c"
-                  proof (atomize_elim, cases upd_op)
-                    case (Author a)
-                    obtain x where "a = Assign x"
-                      using upd_is_update Author 
-                      by (cases a, auto simp add: is_update_messageDataOp_def)
-
-                    show "\<exists>upda_c upda_val.
-                   s_calls' upda_c \<triangleq> Call (Message (NestedOp (MessageId m) (Author (Assign upda_val)))) Undef \<and>
-                   ((upda_c, upd_c) \<in> s_happensBefore' \<or> upda_c = upd_c)"
-                      using Author \<open>a = Assign x\<close> upd_call \<open>upd_r = Undef\<close> by blast
-
-                  next
-                    case (Content a)
-                    obtain x where "a = Assign x"
-                      using upd_is_update Content 
-                      by (cases a, auto simp add: is_update_messageDataOp_def)
-
-                    show "\<exists>upda_c upda_val.
-                 s_calls' upda_c \<triangleq> Call (Message (NestedOp (MessageId m) (Author (Assign upda_val)))) Undef \<and>
-                 ((upda_c, upd_c) \<in> s_happensBefore' \<or> upda_c = upd_c)"
-                      using i3 Content \<open>a = Assign x\<close> \<open>upd_r = Undef\<close> upd_call 
-                      by (auto simp add: inv3_def, blast)
-                  qed
-
-                  have [simp]: "upda_c \<noteq> c"
-                    by (metis Exists_AtReturn(9) inv1(12) invariantContext.simps(1) operationContext.simps(1) option.simps(3) upda_call wellFormed_callOrigin_dom3)
-
-                  from \<open>crdtSpec (Message (NestedOp (MessageId m) (Author Read)))
-                   \<lparr>calls = (s_calls' |` (vis'))(c \<mapsto> Call (Message (KeyExists (MessageId m))) (Bool True)),
-                      happensBefore = updateHb (s_happensBefore' |r vis') vis' [c]\<rparr>
-                   resa\<close>
-                  have spec1: "crdtSpec' (Message (NestedOp (MessageId m) (Author Read))) (insert c (dom s_calls' \<inter> (vis' )))
-                       (extract_op ((s_calls' |` (vis'))(c \<mapsto> Call (Message (KeyExists (MessageId m))) (Bool True))))
-                       (updateHb (s_happensBefore' |r vis') vis' [c]) id resa"
-                    apply (subst(asm) crdtSpec'_alt)
-                  proof (auto simp add: crdtSpec'_alt crdtSpec'_simp_op crdtSpec'_simp_hb  )
-
-                    show "\<exists>y. s_calls' x \<triangleq> y"
-                      if c0: "x \<in> Field (updateHb (s_happensBefore' |r vis') vis' [c])"
-                        and c1: "x \<noteq> c"
-                      for  x
-                      using that `vis' \<subseteq> dom s_calls'` by (auto simp add: in_sequence_cons Field_def restrict_relation_def updateHb_cases)
-
-
-                    show "x \<in> vis'"
-                      if c0: "x \<in> Field (updateHb (s_happensBefore' |r vis') vis' [c])"
-                        and c1: "x \<noteq> c"
-                      for  x
-                      using that `vis' \<subseteq> dom s_calls'` by (auto simp add: in_sequence_cons Field_def restrict_relation_def updateHb_cases)
-
-                  qed
-
-                  have spec2: "crdtSpec' (Message (NestedOp (MessageId m) (Author Read))) 
-                       (insert c (dom s_calls' \<inter> (vis')))
-                       ((extract_op s_calls')(c := Message (KeyExists (MessageId m))))
-                       (updateHb s_happensBefore' vis' [c]) id resa"
-                  proof (rule use_ccrdtSpec_wf1[OF crdtSpec'_wf, rotated -1, OF spec1])
-
-                    show " map_same_on (insert c (dom s_calls' \<inter> (vis' )))
-                       (extract_op ((s_calls' |` (vis' ))(c \<mapsto> Call (Message (KeyExists (MessageId m))) (Bool True))))
-                       ((extract_op s_calls')(c := Message (KeyExists (MessageId m))))"
-                      by (auto simp add: map_same_on_def extract_op_def)
-
-                    show " rel_same_on (insert c (dom s_calls' \<inter> (vis'))) (updateHb (s_happensBefore' |r vis') vis' [c])
-                           (updateHb s_happensBefore' vis' [c])"
-                      using inv1(14) by (auto simp add: rel_same_on_def updateHb_cons restrict_relation_def)
-                  qed
-
-                  have [simp]: "(\<lambda>x. Message (NestedOp (MessageId m) x)) \<circ> Author
-                      = Message \<circ> (NestedOp (MessageId m)) \<circ> Author"
-                    by auto
-
-                  have [simp]: "upda_c \<in> vis'"
-                    using causallyConsistent_def inv1(6) upd_vis upda_before_upd by fastforce
-
-                  from spec2
-                  have "is_from (String author) Undef
-                     (latest_values'
-                       (C_out_calls (Message \<circ> NestedOp (MessageId m) \<circ> Author)
-                         ((extract_op s_calls')(c := Message (KeyExists (MessageId m))))
-                         (C_out_calls (Message \<circ> NestedOp (MessageId m)) ((extract_op s_calls')(c := Message (KeyExists (MessageId m))))
-                           (insert c (dom s_calls' \<inter> (vis'))) -
-                          deleted_calls_dw'
-                           (C_out_calls Message ((extract_op s_calls')(c := Message (KeyExists (MessageId m))))
-                             (insert c (dom s_calls' \<inter> (vis'))))
-                           ((extract_op s_calls')(c := Message (KeyExists (MessageId m)))) (updateHb s_happensBefore' vis' [c]) Message
-                           (MessageId m)))
-                       ((extract_op s_calls')(c := Message (KeyExists (MessageId m)))) (updateHb s_happensBefore' vis' [c])
-                       (Message \<circ> NestedOp (MessageId m) \<circ> Author))"
-                    by (auto simp add: crdtSpec'_def `resa = String author` struct_field'_def map_dw_spec'_def
-                        map_spec'_def restrict_calls_def2 messageStruct'_def register_spec'_def)
-
-                  hence spec3: "(String author) \<in>
-                     (latest_values'
-                       (C_out_calls (Message \<circ> NestedOp (MessageId m) \<circ> Author)
-                         ((extract_op s_calls')(c := Message (KeyExists (MessageId m))))
-                         (C_out_calls (Message \<circ> NestedOp (MessageId m)) ((extract_op s_calls')(c := Message (KeyExists (MessageId m))))
-                           (insert c (dom s_calls' \<inter> (vis' ))) -
-                          deleted_calls_dw'
-                           (C_out_calls Message ((extract_op s_calls')(c := Message (KeyExists (MessageId m))))
-                             (insert c (dom s_calls' \<inter> (vis' ))))
-                           ((extract_op s_calls')(c := Message (KeyExists (MessageId m)))) (updateHb s_happensBefore' vis' [c]) Message
-                           (MessageId m)))
-                       ((extract_op s_calls')(c := Message (KeyExists (MessageId m)))) (updateHb s_happensBefore' vis' [c])
-                       (Message \<circ> NestedOp (MessageId m) \<circ> Author))"
-                    apply (rule is_from_exists[THEN iffD1, rotated])
-                  proof (rule latest_values'_exists)
-
-                    show "finite
-                       (C_out_calls (Message \<circ> NestedOp (MessageId m) \<circ> Author) ((extract_op s_calls')(c := Message (KeyExists (MessageId m))))
-                         (C_out_calls (Message \<circ> NestedOp (MessageId m)) ((extract_op s_calls')(c := Message (KeyExists (MessageId m))))
-                           (insert c (dom s_calls' \<inter> (vis'))) -
-                          deleted_calls_dw'
-                           (C_out_calls Message ((extract_op s_calls')(c := Message (KeyExists (MessageId m))))
-                             (insert c (dom s_calls' \<inter> (vis'))))
-                           ((extract_op s_calls')(c := Message (KeyExists (MessageId m)))) (updateHb s_happensBefore' vis' [c]) Message
-                           (MessageId m)))"
-                    proof (rule finite_subset)
-                      show "finite (dom s_calls')"
-                        using Exists_AtReturn(9) wf_finite_calls by force
-                    qed (auto simp add: C_out_calls_def)
-
-                    have "acyclic s_happensBefore'"
-                      using happensBefore_acyclic[OF local.inv1(17)] by simp
-
-                    show "acyclic (updateHb s_happensBefore' vis' [c])"
-                      using \<open>acyclic s_happensBefore'\<close>
-                      proof (rule acyclic_updateHb)
-
-                        show "distinct [c]" by simp
-
-                        show "vis' \<inter> set [c] = {}"
-                          using \<open>c \<notin> vis'\<close> by auto
-
-                        show " Field s_happensBefore' \<inter> set [c] = {}"
-                          by (metis DomainE Field_def RangeE Un_iff disjoint_iff_not_equal empty_set inv1(14) inv1(15) list.simps(15) singletonD)
-                      qed
-
-                    from upda_before_upd
-                    have delete_before_upda_c: "(d, upda_c) \<in> s_happensBefore'"
-                      if d_not_c: "d \<noteq> c"
-                        and d_vis: "d \<in> vis'"
-                        and d_call: "s_calls' d \<triangleq> Call (Message (DeleteKey (MessageId m))) x2"
-                      for  d x2
-                    proof 
-
-
-                      obtain d_ctxt where "querySpec progr (Message (DeleteKey (MessageId m))) d_ctxt x2"
-                        by (meson d_call get_query_spec inv1(17))
-
-                      hence [simp]: "x2 = Undef"
-                        by (auto simp add: crdtSpec_def struct_field_def map_dw_spec_def map_spec_def) 
-
-                      have [simp]: "d \<in> dom s_calls'"
-                        using d_call by blast
-
-                      have "(d, upd_c) \<in> s_happensBefore'"
-                        using ud_not_deleted[rule_format, where d=d]  d_vis d_call
-                        by (auto simp add: extract_op_def split: option.splits)
-
-                      show "(d, upda_c) \<in> s_happensBefore'" if "upda_c = upd_c"
-                        using `(d, upd_c) \<in> s_happensBefore'` `upda_c = upd_c` by simp
-
-
-                      show "(d, upda_c) \<in> s_happensBefore'"
-                        if c0: "(upda_c, upd_c) \<in> s_happensBefore'"
-                      proof (rule ccontr)
-                        assume "(d, upda_c) \<notin> s_happensBefore'"
-
-                        from `inv4 s_calls' s_happensBefore'`
-                        show False
-                          apply (auto simp add: inv4_def)
-                          apply (drule spec[where x=upd_c])
-                          apply (drule spec[where x=d])
-                          using upd_is_update by (auto simp add: d_call upd_call  \<open>upd_r = Undef\<close> \<open>(d, upd_c) \<in> s_happensBefore'\<close>)
-                      qed
-                    qed
-
-                    show "\<exists>ca y.
-                           ca \<in> C_out_calls (Message \<circ> NestedOp (MessageId m) \<circ> Author)
-                                  ((extract_op s_calls')(c := Message (KeyExists (MessageId m))))
-                                  (C_out_calls (Message \<circ> NestedOp (MessageId m)) ((extract_op s_calls')(c := Message (KeyExists (MessageId m))))
-                                    (insert c (dom s_calls' \<inter> vis')) -
-                                   deleted_calls_dw'
-                                    (C_out_calls Message ((extract_op s_calls')(c := Message (KeyExists (MessageId m))))
-                                      (insert c (dom s_calls' \<inter> vis')))
-                                    ((extract_op s_calls')(c := Message (KeyExists (MessageId m)))) (updateHb s_happensBefore' vis' [c]) Message
-                                    (MessageId m)) \<and>
-                           ((extract_op s_calls')(c := Message (KeyExists (MessageId m)))) ca =
-                           (Message \<circ> NestedOp (MessageId m) \<circ> Author) (Assign y)"
-                    proof (auto simp add: C_out_calls_def cong: conj_cong; intro exI conjI)
-                      show "upda_c \<noteq> c"
-                        by auto
-
-                      from `s_calls' upda_c \<triangleq> Call (Message (NestedOp (MessageId m) (Author (Assign upda_val)))) Undef`
-                      show "extract_op s_calls' upda_c = Message (NestedOp (MessageId m) (Author (Assign upda_val)))"
-                        by (auto  simp add: extract_op_def)
-                      thus "extract_op s_calls' upda_c = Message (NestedOp (MessageId m) (Author (Assign upda_val)))" .
-                      thus "extract_op s_calls' upda_c = Message (NestedOp (MessageId m) (Author (Assign upda_val)))" .
-
-                      show "upda_c \<in> dom s_calls'"
-                        using upda_call by blast
-
-                      show "upda_c \<in> vis'"
-                        by auto
-
-                      show "upda_c
-                          \<notin> deleted_calls_dw' {ca. ca \<noteq> c \<longrightarrow> ca \<in> dom s_calls' \<and> ca \<in> vis' \<and> (\<exists>x. extract_op s_calls' ca = Message x)}
-                        ((extract_op s_calls')(c := Message (KeyExists (MessageId m)))) (updateHb s_happensBefore' vis' [c]) Message
-                        (MessageId m)"
-                        using delete_before_upda_c  by (auto simp add: deleted_calls_dw'_def updateHb_cons extract_op_def' split: call.splits)
-                    qed
-                  qed
-
-                  have [simp]: "c' \<noteq> c" if "c' \<in> vis'" for c'
-                    using \<open>c \<notin> vis'\<close> that by blast
-
-                  have [simp]: "c \<in> dom s_calls'" if "c \<in> vis'" for c
-                    using inv1(4) that by blast
-
-
-                  from spec3
-                  obtain updb_c updb_res
-                    where updb_c1: "\<forall>x. x \<in> dom s_calls' \<longrightarrow> (\<exists>res. s_calls' x \<triangleq> Call (Message (DeleteKey (MessageId m))) res) \<longrightarrow> x \<in> vis' \<longrightarrow> (x, updb_c) \<in> s_happensBefore'"
-                      and updb_c_vis: "updb_c \<in> vis'"
-                      and updb_c_call: "s_calls' updb_c \<triangleq> Call (Message (NestedOp (MessageId m) (Author (Assign (String author))))) updb_res"
-                      and updb_c2: "\<forall>c'. c' \<in> vis' \<longrightarrow> (\<forall>y res. s_calls' c' \<noteq> Some (Call (Message (NestedOp (MessageId m) y)) res)) \<or> (\<exists>y res. s_calls' c' \<triangleq> Call (Message y) res) \<and> (\<exists>x. (\<exists>res. s_calls' x \<triangleq> Call (Message (DeleteKey (MessageId m))) res) \<and> x \<in> vis' \<and> (x, c') \<notin> s_happensBefore') \<or> (\<forall>y res. s_calls' c' \<noteq> Some (Call (Message (NestedOp (MessageId m) (Author y))) res)) \<or> (\<forall>v' res. s_calls' c' \<noteq> Some (Call (Message (NestedOp (MessageId m) (Author (Assign v')))) res)) \<or> (updb_c, c') \<notin> s_happensBefore'"
-                    apply (auto simp add: latest_values'_def latest_assignments'_def in_deleted_calls_dw'
-                      in_C_out extract_op_eq Ball_def Bex_def updateHb_cons
-                        split: if_splits
-                      cong: conj_cong disj_cong
-                      )
-                    by blast
-
-                  from updb_c_call
-                  have "\<exists>ctxt. querySpec progr (Message (NestedOp (MessageId m) (Author (Assign (String author))))) ctxt updb_res"
-                    by (meson get_query_spec inv1(17))
-
-                  hence [simp]: " updb_res = Undef"
-                    by (auto simp add: crdtSpec_def struct_field_def map_dw_spec_def map_spec_def messageStruct_def register_spec_def)
-
-                  from updb_c_call
-                  have updb_c_call': " s_calls' updb_c \<triangleq> Call (Message (NestedOp (MessageId m) (Author (Assign (String author))))) Undef"
-                    by simp
-
-                  from `inv2 (s_invocationOp'(i \<mapsto> GetMessage m)) s_calls'`[unfolded inv2_def, rule_format, OF updb_c_call']
-                  obtain ia s where "(s_invocationOp'(i \<mapsto> GetMessage m)) ia \<triangleq> SendMessage author s"
-                    by blast
-
-                  thus "\<exists>s. s \<noteq> i \<and> (\<exists>content2. s_invocationOp' s \<triangleq> SendMessage author content2)"
-                    by (metis map_upd_Some_unfold proc.distinct(5))
-                qed
-              qed
-            qed
-          next
-            case (NotExists_AtCommit tx s_calls' s_happensBefore' s_callOrigin' s_transactionOrigin' s_knownIds' vis' s_invocationOp' s_invocationRes' c res)
-            then show ?case
-            proof (auto simp add: inv_def, goal_cases inv2 inv3 inv4)
-              case (inv2 some_generatedIds some_generatedIds1 some_currentTransaction some_currentTransaction1 some_localState some_localState1 some_currentProc some_currentProc1 some_visibleCalls some_visibleCalls1 some_transactionStatus some_transactionStatus1 some_generatedIds2 some_currentTransaction2 some_localState2 some_currentProc2 some_visibleCalls2 some_transactionStatus2)
-              then show ?case 
-                by (auto simp add: inv2_def)
-            next
-              case (inv3 some_generatedIds some_generatedIds1 some_currentTransaction some_currentTransaction1 some_localState some_localState1 some_currentProc some_currentProc1 some_visibleCalls some_visibleCalls1 some_transactionStatus some_transactionStatus1 some_generatedIds2 some_currentTransaction2 some_localState2 some_currentProc2 some_visibleCalls2 some_transactionStatus2)
-              then show ?case 
-                by (auto simp add: inv3_def updateHb_cases in_sequence_cons cong: conj_cong, fastforce)
-            next
-              case (inv4 some_generatedIds some_generatedIds1 some_currentTransaction some_currentTransaction1 some_localState some_localState1 some_currentProc some_currentProc1 some_visibleCalls some_visibleCalls1 some_transactionStatus some_transactionStatus1 some_generatedIds2 some_currentTransaction2 some_localState2 some_currentProc2 some_visibleCalls2 some_transactionStatus2)
-              then show ?case 
-                by (auto simp add: inv4_def updateHb_cases in_sequence_cons)
-            qed
-          next
-            case (NotExists_AtReturn tx s_calls' s_happensBefore' s_callOrigin' s_transactionOrigin' s_knownIds' vis' s_invocationOp' s_invocationRes' c res)
-            then show ?case
-              apply (auto simp add: inv_def)
-              apply (auto simp add: inv1_def)
-              by (metis (no_types, lifting) option.inject proc.distinct(5))
-          qed
-        qed
+        qed (auto simp add: finalCheck_def)
       qed
     qed
   qed
 qed
+
 
 
 end
